certicoq/theories/L2_5_box/stripEvalCommute.v
@@ -1,3 +1,4 @@
+
 Require Import Coq.Lists.List.
 Require Import Coq.Strings.String.
 Require Import Coq.Strings.Ascii.
@@ -32,10 +33,10 @@ Definition optStrip (t:option L2Term) : option Term :=
     | None => None
     | Some t => Some (strip t)
   end.
-Definition optStrips (ts:option L2Terms) : option Terms :=
+Definition optL2Terms_Terms (ts:option L2Terms) : option Terms :=
   match ts with
     | None => None
-    | Some ts => Some (strips ts)
+    | Some ts => Some (L2Terms_Terms ts)
   end.
 Definition optStripDnth (b: option (L2Term * nat)) : option (Term * nat) :=
                            match b with
@@ -46,13 +47,13 @@ Definition optStripCanP
            (b: option (nat * L2Terms * nat)): option (nat * Terms * nat) :=
                            match b with
                              | None => None
-                             | Some (n, t, m) => Some (n, strips t, m)
+                             | Some (n, t, m) => Some (n, L2Terms_Terms t, m)
                            end.
 
 Lemma optStrip_hom: forall y, optStrip (Some y) = Some (strip y).
 induction y; simpl; reflexivity.
 Qed.
-Lemma optStrips_hom: forall y, optStrips (Some y) = Some (strips y).
+Lemma optL2Terms_Terms_hom: forall y, optL2Terms_Terms (Some y) = Some (L2Terms_Terms y).
 induction y; simpl; reflexivity.
 Qed.
 Lemma optStripDnth_hom:
@@ -60,11 +61,10 @@ Lemma optStripDnth_hom:
 induction y; simpl; reflexivity.
 Qed.
 Lemma optStripCanP_hom:
-  forall y n m, optStripCanP (Some (n, y, m)) = Some (n, strips y, m).
+  forall y n m, optStripCanP (Some (n, y, m)) = Some (n, L2Terms_Terms y, m).
 induction y; simpl; reflexivity.
 Qed.
                               
-Print L2Env.
 Lemma Lookup_hom:
   forall (p:environ L2.compile.Term) s ec, Lookup s p ec -> Lookup s (L2Env_Env p) (L2EC_EC ec).
 Proof.
@@ -79,10 +79,49 @@ Proof.
   - cbn. apply LMiss; assumption.
 Qed.
 
+Lemma lookup_hom:
+  forall p nm ec,
+    lookup nm p = Some ec -> lookup nm (stripEnv p) = Some (L2EC_EC ec).
+Proof.
+  intros p nm ec h. apply Lookup_lookup.
+  apply Lookup_hom. apply (lookup_Lookup _ _ h).
+Qed.
+  
+Lemma lookup_hom_None:
+  forall p nm,
+    lookup nm p = None -> lookup nm (L2Env_Env p) = None.
+Proof.
+  induction p; intros.
+  - cbn. reflexivity.
+  - destruct a. destruct (string_dec nm s).
+    + subst. cbn in H. rewrite string_eq_bool_rfl in H. discriminate.
+    + cbn. rewrite (string_eq_bool_neq n).
+      cbn in H. rewrite (string_eq_bool_neq n) in H.
+      apply IHp. assumption.
+Qed.
+
 Lemma LookupDfn_hom:
  forall p s t, LookupDfn s p t -> LookupDfn s (stripEnv p) (strip t).
 unfold LookupDfn. intros.
 assert (j:= Lookup_hom H). exact j.
+Qed.
+
+Lemma lookupDfn_hom:
+  forall p nm t,
+    lookupDfn nm p = Ret t -> lookupDfn nm (stripEnv p) = Ret (strip t).
+Proof.
+  induction p; intros.
+  - cbn in *. discriminate.
+  - destruct a. unfold lookupDfn. cbn. unfold lookupDfn in H. cbn in H.
+    destruct (string_dec nm s).
+    + subst. cbn. cbn in H.
+      rewrite string_eq_bool_rfl. rewrite string_eq_bool_rfl in H.
+      destruct e; try discriminate.
+      * myInjection H. cbn. reflexivity.
+    + rewrite (string_eq_bool_neq n). rewrite (string_eq_bool_neq n) in H.
+      case_eq (lookup nm p); intros; rewrite H0 in H; try discriminate.
+      * rewrite (lookup_hom _ _ H0). destruct e0; try discriminate.
+        cbn. myInjection H. reflexivity.
 Qed.
 
 Lemma dlength_hom:
@@ -91,11 +130,12 @@ induction ds. intuition. simpl. rewrite IHds. reflexivity.
 Qed.
 
 Lemma tcons_hom:
-  forall t ts, strips (L2.compile.tcons t ts) = tcons (strip t) (strips ts).
+  forall t ts, L2Terms_Terms (L2.compile.tcons t ts) =
+               tcons (strip t) (L2Terms_Terms ts).
 reflexivity.
 Qed.
 
-Lemma tnil_hom: strips L2.compile.tnil = tnil.
+Lemma tnil_hom: L2Terms_Terms L2.compile.tnil = tnil.
 reflexivity.
 Qed.
 
@@ -116,3 +156,191 @@ Lemma dnthBody_hom:
 induction m; induction ds; try intuition.
 - simpl. intuition.
 Qed.
+
+Lemma tappend_hom:
+  forall ts us,
+    L2Terms_Terms (L2.term.tappend ts us) =
+    tappend (L2Terms_Terms ts) (L2Terms_Terms us).
+induction ts; intros us; simpl. reflexivity.
+rewrite IHts. reflexivity.
+Qed.
+
+Lemma TApp_hom:
+  forall fn arg args,
+    strip (L2.compile.TApp fn arg args) =
+    TApp (strip fn) (strip arg) (strips args).
+induction fn; intros arg args; try reflexivity.
+Qed.
+
+
+(*******************
+Lemma isApp_hom:
+  forall t, isApp (strip t) -> L2.term.isApp t.
+Proof.
+  destruct t; cbn; intros h;
+  destruct h as [x0 [x1 [x2 h]]]; try discriminate. 
+  - exists t1, t2, t3. reflexivity.
+  - destruct p as [[y0 y1] y2]. destruct y2.
+    + discriminate.
+    + 
+    destruct t.
+Qed.
+
+Lemma mkApp_hom:
+forall fn args,
+  strip (L2.term.mkApp fn args) = mkApp (strip fn) (L2Terms_Terms args).
+Proof.
+  destruct args; try (reflexivity).
+  - rewrite L2.term.mkApp_tnil_ident. rewrite mkApp_tnil_ident.
+    reflexivity.
+  - destruct fn; try reflexivity.
+    + change (TApp (strip fn1) (strip fn2)
+                   (strips (L2.term.tappend t0 (L2.compile.tcons t args))) =
+              TApp (strip fn1) (strip fn2)
+                   (tappend (strips t0) (tcons (strip t) (strips args)))).
+      rewrite <- tcons_hom. rewrite <- tappend_hom. reflexivity.
+    + rewrite L2.term.mkApp_goodFn. rewrite tcons_hom.
+      rewrite mkApp_goodFn. rewrite TApp_hom. reflexivity.
+      * { induction fn; unfold strip;  
+          intros h; destruct h as [x0 [x1 [x2 jx]]]; cbn in jx;
+          destruct p as [[y0 y1] y2]; try discriminate.
+          - induction t0; cbn in jx.
+            + discriminate.
+            + cbn in jx. 
+            
+      * { intros h. destruct h as [x0 [x1 [x2 jx]]]. cbn in jx.
+          destruct p as [[i k] ks]. destruct fn; cbn in jx; try discriminate.
+          - admit.
+          -
+  -
+      
+      cbn. rewrite tappend_hom. L2Terms_Terms. cbn. rewrite <- tcons_hom. rewrite <- tappend_hom. reflexivity.
+
+
+    destruct fn; cbn.
+    rewrite L1g.term.tappend_tnil. reflexivity.
+  - destruct fn; cbn; try reflexivity.
+  - destruct fn; cbn; try reflexivity.
+  - rewrite tappend_tnil. rewrite L2.term.tappend_tnil. reflexivity.
+  -
+  
+  - rewrite <- tcons_hom. rewrite <- tappend_hom. reflexivity.
+Qed.
+
+  intros fn args. functional induction (L2.term.mkApp fn args).
+  -  cbn.
+  
+
+Lemma instantiate_hom:
+  (forall bod arg n, strip (L2.term.instantiate arg n bod) =
+                     instantiate (strip arg) n (strip bod)) /\
+    (forall bods arg n, L2Terms_Terms (L2.term.instantiates arg n bods) =
+                    instantiates (strip arg) n (L2Terms_Terms bods)) /\
+    (forall ds arg n, stripDs (L2.term.instantiateDefs arg n ds) =
+                      instantiateDefs (strip arg) n (stripDs ds)).
+Proof.
+  apply L2.compile.TrmTrmsDefs_ind; intros; try (simpl; reflexivity).
+  - simpl. destruct (lt_eq_lt_dec n n0); cbn.
+    + destruct s.
+      * rewrite (proj1 (nat_compare_gt n0 n)); try omega. cbn. reflexivity.
+      * subst n. rewrite (proj2 (nat_compare_eq_iff _ _)); trivial.
+        rewrite L2.term.mkApp_tnil_ident. reflexivity.
+    + rewrite (proj1 (nat_compare_lt n0 n)); trivial.
+  - admit.
+  - cbn. rewrite H. reflexivity.
+  - cbn. rewrite H. reflexivity.
+  - cbn. rewrite H. rewrite H0. reflexivity.
+   - change (strip (L2.term.mkApp
+                     (L2.term.instantiate arg n t)
+                     (L2.compile.tcons (L2.term.instantiate arg n t0)
+                                         (L2.term.instantiates arg n t1))) =
+            instantiate (strip arg) n (strip (L2.compile.TApp t t0 t1))). 
+Check TApp_hom. 
+    change
+      (strip (L2.term.mkApp
+                (L2.term.instantiate arg n t)
+                (L2.compile.tcons (L2.term.instantiate arg n t0)
+                                   (L2.term.instantiates arg n t1))) =
+       (mkApp (instantiate (strip arg) n (strip t))
+              (tcons (instantiate (strip arg) n (strip t0))
+                     (instantiates (strip arg) n (L2Terms_Terms t1))))).
+    rewrite <- H. rewrite <- H0. rewrite <- H1. 
+    Check mkApp_hom. rewrite tcons_hom. reflexivity.
+  - change (TCase p (strip (L2.term.instantiate arg n t0))
+                  (L2Terms_Terms (L2.term.instantiates arg n t1)) =
+            (TCase p (instantiate (strip arg) n (strip t0))
+                   (instantiates (strip arg) n (L2Terms_Terms t1)))).
+    rewrite H0. rewrite H1. reflexivity.
+  - change (TFix (stripDs (L2.term.instantiateDefs
+                             arg (n0 + L2.compile.dlength d) d)) n =
+            (TFix (instantiateDefs
+                     (strip arg) (n0 + dlength (stripDs d)) (stripDs d)) n)).
+    rewrite H. rewrite dlength_hom. reflexivity.
+  - change (tcons (strip (L2.term.instantiate arg n t))
+                  (L2Terms_Terms (L2.term.instantiates arg n t0)) =
+            tcons (instantiate (strip arg) n (strip t))
+                  (instantiates (strip arg) n (L2Terms_Terms t0))).
+    rewrite H. rewrite H0. reflexivity.
+  - change (dcons n (strip (L2.term.instantiate arg n1 t0)) n0
+                  (stripDs (L2.term.instantiateDefs arg n1 d)) =
+            dcons n (instantiate (strip arg) n1 (strip t0)) n0
+                  (instantiateDefs (strip arg) n1 (stripDs d))).
+    rewrite H0. rewrite H1. reflexivity.
+Qed.
+
+
+
+Lemma WcbvEval_hom:
+  forall p,
+    (forall t t', L2.wcbvEval.WcbvEval p t t' ->
+                  WcbvEval (stripEnv p) (strip t) (strip t')) /\
+    (forall ts ts', L2.wcbvEval.WcbvEvals p ts ts' ->
+                    WcbvEvals (stripEnv p) (L2Terms_Terms ts) (strips ts')).
+Proof.
+  intros p.
+  apply L2.wcbvEval.WcbvEvalEvals_ind; intros; try reflexivity;
+  try (solve[ constructor; intuition]).  
+  - cbn. destruct t; cbn; try (try constructor; assumption).
+  - cbn. econstructor; try eassumption.
+    eapply (lookupDfn_hom). assumption.
+(*************
+  - destruct (L2.term.isApp_dec t).
+    + destruct i as [x0 [x1 [x2 jx]]]. subst t. 
+      cbn. econstructor. eapply H. intros h. discriminate.
+    + cbn. destruct t; cbn; try (solve[eapply H; intros k; discriminate]).
+      
+    + unfold isProof in H1. rewrite H1 in H0. cbn in H0.
+    
+    destruct H0 as [u ju]. subst t. cbn. inversion_Clear w.
+**********)
+  - cbn. eapply wAppLam.
+    + apply H. 
+    + apply H0. 
+    + rewrite whBetaStep_hom in H1. assumption.
+  - cbn. eapply wLetIn.
+    + apply H. 
+    + rewrite <- (proj1 instantiate_hom). assumption.
+  - cbn. eapply wAppFix.
+    + eapply H.
+    + apply H0.
+    + rewrite <- dnthBody_hom. rewrite e. reflexivity.
+    + rewrite tlength_hom. assumption.
+    + rewrite <- pre_whFixStep_hom in H1. eapply H1.
+  - destruct (WcbvEvals_tcons_tcons H0) as [a' [args' j]]. rewrite j in H0.
+    cbn. rewrite mkApp_hom. eapply wAppCong. try eassumption.
+    + intros h. elim n. apply isLambda_hom. assumption.
+    + intros h. elim n0. apply isFix_hom. assumption.
+    + rewrite j. cbn in H0. assumption.
+  - cbn. eapply wAppFixCong1; try eassumption.
+    + rewrite <- dnthBody_hom. rewrite e. reflexivity.
+    + rewrite tlength_hom. assumption. 
+  - refine (wCase _ _ _ _ _ _ _); try eassumption.
+    * rewrite <- canonicalP_hom. rewrite e. reflexivity.
+    * rewrite <- tskipn_hom. rewrite e0. reflexivity.
+    * rewrite <- whCaseStep_hom. rewrite e1. reflexivity.
+  - refine (wCaseCong _ _ _ _); try eassumption.
+    + rewrite <- canonicalP_hom. rewrite e. reflexivity.
+Qed.
+Print Assumptions WcbvEval_hom.
+
+****************************)
